Change internal representation of Buffer, simplify Buffer.live

ulib/ml/FStar_Buffer.ml
@@ -51,3 +51,5 @@ let only a = BatSet.empty
 
 let op_Array_Access b n = index b n
 let op_Array_Assignment b n v = upd b n v
+
+let recall = fun b -> ()
